Strata/DL/Lambda/LTyUnify.lean
@@ -144,6 +144,7 @@ def LMonoTy.subst (S : Subst) (mty : LMonoTy) : LMonoTy :=
   match mty with
   | .ftvar x => match S.find? x with
                 | some sty => sty | none => mty
+  | .bitvec _ => mty
   | .tcons name ltys r =>
     .tcons name (LMonoTys.subst S ltys) r
 /--
@@ -218,6 +219,10 @@ theorem LMonoTy.subst_keys_not_in_substituted_type (h : SubstWF S) :
       have := @Map.find?_of_not_mem_values _ _ i _ S
       simp_all
       exact ne_of_mem_of_not_mem hid this
+  case bitvec n =>
+    simp_all [LMonoTy.subst]
+    unfold LMonoTy.freeVars
+    simp
   case tcons name args r h1 =>
     simp_all
     simp [subst]
@@ -259,6 +264,8 @@ theorem LMonoTy.freeVars_of_subst_subset (S : Subst) (mty : LMonoTy) :
       apply @Map.find?_mem_values _ _ x sty _ S h_find
     · -- Case: S.find? x = none
       simp [freeVars]
+  case bitvec n =>
+    simp [subst]
   case tcons name args r ih =>
     simp [LMonoTy.subst, LMonoTy.freeVars]
     induction args
